\documentclass{beamer}
\usepackage{amsmath,amsfonts,amsthm,amstext,amssymb, xcolor, tikz, pgf}

% ----------------------------------------------------------
% Theme Setup

% Use Metropolis Theme
\usetheme[numbering=fraction]{metropolis}
\setbeamertemplate{blocks}[rounded][shadow=false]
\makeatletter
\setlength{\metropolis@titleseparator@linewidth}{1pt}
\makeatother



% Define Colors
\definecolor{chargerblue}{HTML}{002764}
\definecolor{chargerred}{HTML}{e02034}
\definecolor{bggray}{HTML}{d0d3d4}

% Set Colors
\setbeamercolor{title}{fg=chargerblue}
\setbeamercolor{background canvas}{bg=white}
\setbeamercolor{title separator}{fg=chargerred}
\setbeamercolor{structure}{fg=chargerblue}
\setbeamercolor{frametitle}{fg=white, bg=chargerblue}
\setbeamercolor*{normal text}{fg=chargerblue}
\setbeamercolor*{block body}{bg=bggray}
\setbeamercolor*{block title}{bg=chargerblue, fg=white}
% ----------------------------------------------------------

% ----------------------------------------------------------
% Custom Definitions, Commands, Environments, etc.

% Sets of numbers
\def\R{\mathbb{R}} % The reals
\def\N{\mathbb{N}} % The naturals
\def\Z{\mathbb{Z}} % The integers
\def\Q{\mathbb{Q}} % The rationals

% Blank space
\newcommand{\blank}[1]{\underline{\hspace{#1}}} % Blank space

% Fitted inclusion symbols
\newcommand{\fp}[1]{\left({#1}\right)} % Fitted parentheses around content
\newcommand{\fb}[1]{\left[{#1}\right]} % Fitted brackets
\newcommand{\set}[1]{\left\{{#1}\right\}} % Fitted braces (useful for sets)
\newcommand{\av}[1]{\left|{#1}\right|} % Fitted absolute value bars

% Coordinate Plane (Four-Quadrant)
\def\coordplane {
	\begin{tikzpicture}
		\draw[step=0.25cm,black,very thin,opacity=0.25] (-2.5cm, -2.5cm) grid (2.5cm, 2.5cm);
		\draw[<->,thick,black] (-2.5cm, 0) -- (2.5cm, 0) node[anchor=north west,pos=0.94,font=\scriptsize]{$x$};
		\draw[<->,thick,black] (0,-2.5cm) -- (0, 2.5cm) node[anchor=south east,font=\scriptsize,pos=0.94]{$y$};
	\end{tikzpicture}
}

% Coordinate Plane (One-Quadrant)
\def\onequad {
	\begin{tikzpicture}
		\draw[step=0.25cm, black, very thin, opacity=0.25] (0,0) grid (7.5cm,5cm);
		\draw[->, thick, black] (0,0) -- (7.5cm, 0) node[anchor=north west,font=\scriptsize,pos=0.94]{$x$};
		\draw[->, black, thick] (0,0) -- (0,5cm) node[anchor=south east,font=\scriptsize,pos=0.94]{$y$};
	\end{tikzpicture}
}
% ----------------------------------------------------------


% ----------------------------------------------------------
% Presentation Information 
\title[2.6 and 2.7]{Operations with Functions; Inverse Functions}
\subtitle{Sections 2.6 and 2.7}
\author{Jacob Ayers}
\institute{Lesson \#10}
\date{MAT 130}
% ----------------------------------------------------------

\begin{document}

% Slide 1 (Title Slide)
\begin{frame}
\titlepage
\end{frame}

% Slide 2 (Objectives)
\begin{frame}[t]{Objectives}
\begin{itemize}
	\item Add, subtract, multiply, and divide functions
	\item Compose Functions
	\item Verify inverse functions graphically and algebraically
	\item Use the Horizontal Line Test to determine whether a function is one-to-one
	\item Find inverse functions algebraically
\end{itemize}

\end{frame}\begin{frame}[t]{Operations with Functions}
\begin{block}{Sum, Difference, Product, Quotient of Functions}
Let $f$ and $g$ be functions with overlapping domains. Then for all $x$ common to both domains, the sum, difference, product and quotient of $f$ and $g$ are defined as follows:

Sum: $(f + g)(x) = f(x) + g(x)$ \vspace{12pt}

Difference: $(f - g)(x) = f(x) - g(x)$ \vspace{12pt}

Product: $(fg)(x) = f(x) \cdot g(x)$ \vspace{12pt}

Quotient: $\fp{\dfrac{f}{g}}(x) = \dfrac{f(x)}{g(x)} \; \text{ provided } g(x) \neq 0$
\end{block}
\end{frame}

\begin{frame}[t]{Operations with Functions}
Suppose that $f(x) = x^2 + 6x + 5$ and $g(x) = x^2 - 4x - 21$. Find $(f + g)(x)$ and $(g - f)(x)$.
\begin{flalign*}
\onslide<2->{(f+g)(x) &= f(x) + g(x) & \\}
\onslide<3->{&= \fp{x^2 + 6x + 5} + \fp{x^2 - 4x - 21} & \\}
\onslide<4->{&= 2x^2 + 2x - 16}
\end{flalign*}

\begin{flalign*}
\onslide<5->{(g-f)(x) &= g(x) - f(x) & \\}
\onslide<6->{&= \fp{x^2 - 4x - 21} - \fp{x^2 + 6x + 5} & \\}
\onslide<7>{&= -10x - 26}
\end{flalign*}
\end{frame}

\begin{frame}[t]{Operations with Functions}
Suppose that $f(x) = x^2 - 1$ and $g(x) = x - 1$. Find $(fg)(x)$ and $\fp{\dfrac{f}{g}}(x)$.
\begin{flalign*}
\onslide<2->{(fg)(x) &= f(x)\cdot g(x) & \\}
\onslide<3->{&= \fp{x^2 - 1}\fp{x - 1} & \\}
\onslide<4->{&= x^3 - x^2 - x + 1}
\end{flalign*}

\begin{flalign*}
\onslide<5->{\fp{\dfrac{f}{g}}(x) &= \dfrac{f(x)}{g(x)} & \\}
\onslide<6->{&= \dfrac{x^2 - 1}{x - 1} & \\}
\onslide<7->{&= \dfrac{(x+1)(x-1)}{x-1)} & \\}
\onslide<8>{&= x + 1; \; \text{ } x \neq 1}
\end{flalign*}
\end{frame}

\begin{frame}[t]{Composing Functions}
\begin{block}{Definition}
The \textit{composition} of the function $f$ with the function $g$ is \vspace{-8pt} $$(f\circ g)(x) = f\fb{g(x)}$$ \vspace{-8pt}
\end{block}

\pause

\includegraphics[width=4in]{CompIllustration.png}
\end{frame}

\begin{frame}[t]{Composing Functions}
Suppose that $f(x) = 2x + 5$ and $g(x) = 4x^2 + 1$. Find $f\circ g$ and $g\circ f$
\begin{flalign*}
\onslide<2->{f\circ g &= f\fb{g(x)} & \\}
\onslide<3->{&= f\fb{4x^2 + 1} & \\}
\onslide<4->{&= 2\fp{4x^2 + 1} + 5 & \\}
\onslide<5->{&= 8x^2 + 7}
\end{flalign*}
\begin{flalign*}
\onslide<6->{g\circ f &= g\fb{f(x)} & \\}
\onslide<7->{&= g\fb{2x+5} & \\}
\onslide<8->{&= 4\fp{2x+5}^2 + 1 & \\}
\onslide<9->{&= 4\fp{4x^2 + 20x + 25} + 1 & \\}
\onslide<10>{&= 16x^2 + 80x + 101}
\end{flalign*}
\end{frame}

\begin{frame}[t]{Composing Functions}
Suppose that $f(x) = \sqrt{x-2}$ and $g(x) = x^2 + 2$. Find $f\circ g$ and $g\circ f$.
\begin{flalign*}
\onslide<2->{f\circ g &= f\fb{g(x)} & \\}
\onslide<3->{&= f\fb{x^2 + 2} & \\}
\onslide<4->{&= \sqrt{x^2 + 2 - 2} & \\}
\onslide<5->{&= \sqrt{x^2} = x}
\end{flalign*} 
\begin{flalign*}
\onslide<6->{g\circ f &= g\fb{f(x)} & \\}
\onslide<7->{&= g\fb{\sqrt{x-2}} & \\}
\onslide<8->{&= \fp{\sqrt{x-2}}^2 + 2 & \\}
\onslide<9>{&= x-2+2 = x}
\end{flalign*}
\end{frame}

\begin{frame}[t]{An Application}
The number $N$ of bacteria in a refrigerated food is given by $$N(T) = 8T^2 - 14T + 200, 2\leq T\leq 12$$ where $T$ is the temperature of the food in degrees Celsius. When the food is removed from refrigeration, the temperature of the food is given by $$T(t) = 2t+2, 0\leq t \leq 5$$ where $t$ is the time in hours. \begin{enumerate}[(a)]
\item Find and interpret $N\circ T$
\item Find the time when the bacteria count reaches 1000.
\end{enumerate}
\end{frame}

\begin{frame}[t]{An Application}
(a) Find and interpret $N \circ T$.

\pause

Let's start by interpreting the meaning of this composition. This involves looking at the input (domain) and output (range) of each function.

\pause

We know that $N \circ T = N\fb{T(t)}$. Starting with the inner function, $T(t)$: \pause \\
The \textit{input}, $t$, is the time since the food was removed from the refrigerator. \\
The \textit{output}, $T(t)$, is the temperature of the food after $t$ hours.

\pause

Now, moving to the outer function, $N\fb{T(t)}$: \pause \\
The \textit{input}, $T(t)$ is the temperature of the food after $t$ hours. \\
The \textit{output}, $N\fb{T(t)}$, is the number of bacteria at that temperature.
\end{frame}

\begin{frame}[t]{An Application}
Putting it all together: \\ \pause
The initial input is a time in hours, and the final output is a number of bacteria.

\pause

The function $N\circ T$ represents the number of bacteria present $t$ hours after the food was removed from the refrigerator.

\pause

We can now find $N\circ T$: \pause
\begin{flalign*}
N\circ T &= N\fb{T(t)} & \\
&= N\fb{2t + 2} & \\
&= 8\fp{2t+2}^2 - 14\fp{2t+2} + 200 & \\
&= 8\fp{4t^2 + 8t + 4} - 28t - 28 + 200 & \\
&= 32t^2 + 36t + 204
\end{flalign*}
\end{frame}

\begin{frame}[t]{An Application}
(b) Find the time when the bacteria count reaches 1000.

\pause

The variables are time and bacteria count, so we need to use the function $N \circ T$. We want to know when the \textit{output} reaches 1000.
\pause
\begin{flalign*}
1000 &= 32t^2 + 36t + 204 & \\
32t^2 + 36t - 796 &= 0 &
\end{flalign*}
\pause
I trust you could solve that using the Quadratic Formula if you had to, but we'll let Wolfram|Alpha do the work for us here.

\pause

The solutions given are $t \approx 4.4566$ and $t \approx -5.5816$; a negative time makes no sense, so we conclude that there will be 1000 bacteria after about $4.4566$ hr.
\end{frame}

\begin{frame}[t]{Inverse Functions}
We saw earlier that $f\circ g$ and $g\circ f$ might come out to the same answer, and they might not.

\pause

It turns out that functions for which $f\circ g$ and $g\circ f$ are special - they are called \textit{inverses} of one another. \vspace{12pt}

\pause

\includegraphics[width=4in]{InvIllustration.png}
\end{frame}

\begin{frame}[t]{Inverse Functions}
\begin{block}{Definition}
Let $f$ and $g$ be functions such that $f\circ g = g\circ f = x$. \vspace{12pt}

Then $g$ is the \textit{inverse} function of $f$ (and vice versa). We denote $g = f^{-1}$ (read ``$f$-inverse") \vspace{12pt}

So $f\fb{f^{-1}(x)} = f^{-1}\fb{f(x)} = x$. \vspace{12pt}

Note that in order for two functions to be inverses, the domain of $f$ must be the same as the range of $f^{-1}$, and the range of $f$ must be the same as the domain of $f^{-1}$.
\end{block}

\pause

It is important to remember that $f^{-1}$ represents the inverse of $f$, not its reciprocal.
\end{frame}

\begin{frame}[t]{Verifying Inverse Functions Algebraically}
Verify that $f(x) = \dfrac{x-4}{7}$ and $g(x) = 7x + 4$ are inverses of each other.

\onslide<2->{To verify this, we need to confirm that $f\circ g = g\circ f = x}$.
\begin{flalign*}
\onslide<3->{f\fb{g(x)} &= f\fp{7x+4} & \\}
\onslide<4->{&= \dfrac{\fp{7x+4}-4}{7} & \\}
\onslide<5->{&= \dfrac{7x}{7}=x}
\end{flalign*}
\begin{flalign*}
\onslide<6->{g\fb{f(x)} &= g\fp{\dfrac{x-4}{7}} & \\}
\onslide<7->{&= 7\fp{\dfrac{x-4}{7}} + 4 & \\}
\onslide<8>{&= x-4+4 = x}
\end{flalign*}
\end{frame}

\begin{frame}[t]{Verifying Inverse Functions Graphically}
The graphs of $f$ and $f^{-1}$ are related in the following way:
\pause

If $(a,b)$ is on the graph of $f$, then $(b,a)$ is on the graph of $f^{-1}$.

Example: Verify that $f(x) = x^2 + 1 (x\geq 0)$ and $g(x) = \sqrt{x-1}$ are inverses.
\end{frame}

\begin{frame}[t]{One-To-One Functions and HLT}
\begin{block}{Definition}
A function is \textit{one-to-one} if and only if each value of the dependent variable ($y$) maps to exactly one value of the independent variable ($x$). A function $f$ has an inverse if and only if it is one-to-one.
\end{block}

\pause

\begin{block}{Horizontal Line Test}
A function $f$ is one-to-one and has an inverse if and only if no horizontal line intersects its graph more than once.
\end{block}

\pause

Example: Determine whether each function has an inverse: (a) $f(x) = x^2$ and (b) $f(x) = \dfrac12\fp{3-x}$. \pause \\ (a) NO \hspace{1in} (b) YES
\end{frame}

\begin{frame}[t]{Finding Inverse Functions Algebraically}
\begin{block}{Finding an Inverse Function}
\begin{enumerate}[1)]
\item Use HLT to determine if $f$ has an inverse.
\item In the equation for $f(x)$, replace $f(x)$ with $y$.
\item Interchange the roles of $x$ and $y$; solve for $y$.
\item Replace $y$ with $f^{-1}$ in the new equation.
\item Verify that $f\circ f^{-1} = f^{-1}\circ f = x$.
\end{enumerate}
\end{block}
\end{frame}

\begin{frame}[t]{Finding Inverse Functions Algebraically}
Find the inverse function of $f(x) = \dfrac{5-3x}{x+2}$.

\begin{flalign*}
\onslide<2->{y &= \dfrac{5 - 3x}{x+2} & \text{(replace $f(x)$ with $y$)} & \\}
\onslide<3->{x &= \dfrac{5-3y}{y+2} & \text{(interchange $x$ and $y$)} & \\}
\onslide<4->{x(y+2) &= 5 - 3y & \\}
\onslide<5->{xy+2x &=5-3y & \\}
\onslide<6->{xy+3y&=5-2x & \\}
\onslide<7->{y(x+3)&=5-2x & \\}
\onslide<8->{f^{-1} &= \dfrac{5-2x}{x+3} & \text{(solve for $y$, replace $y$ with $f^{-1}$)}}
\end{flalign*}
\end{frame}

\begin{frame}[t]{Finding Inverse Functions Algebraically}
Find the inverse function of $f(x) = \sqrt[3]{10 + x}$

\begin{flalign*}
\onslide<2->{y &= \sqrt[3]{10 + x} & \text{(replace $f(x)$ with $y$)} & \\}
\onslide<3->{x &= \sqrt[3]{10 + y} & \text{(interchange $x$ and $y$)} & \\}
\onslide<4->{x^3 &= 10 + y & \\}
\onslide<5->{f^{-1} &= x^3 - 10 & \text{(solve for $y$, replace $y$ with $f^{-1}$)}}
\end{flalign*}
\end{frame}

\begin{frame}[t]{Next Steps}
\begin{itemize}
\item Prepare for and Take Midterm 1
\begin{itemize}
\item Post questions in Lesson 10 Forum or Midterm 1 Forum, if you have any
\item Work on study guide (NOT a graded assignment)
\item Attend conference Monday night
\item Midterm 1 is Wednesday
\end{itemize}
\item Complete Assignment \#5
\item Begin Module \#7
\begin{itemize}
\item Read 3.1 and 3.2
\item Watch Video Lesson \#11
\end{itemize}
\end{itemize}

\vfill

Thanks for watching!
\end{frame}

\end{document}